pancake/crepLangScript.sml
@@ -47,7 +47,7 @@ Datatype:
        | Call ret ('a exp) (('a exp) list)
        | ExtCall string varname varname varname varname
       (* FFI name, conf_ptr, conf_len, array_ptr, array_len *)
-       | Raise eid ('a exp)
+       | Raise eid
        | Return ('a exp)
        | Tick;
 
